tenvとtableを分離

Typing.v
@@ -1,55 +1,211 @@
 Require Import List.
 Require Import String.
-Require Import FSets.FMapWeakList.
-Require Import FSets.FMapInterface.
-Require Import FSets.FMapFacts.
-Require Import Logic.DecidableType.
 
+Require Import Tables.
 Require Import Term.
 
-(* type *)
-Module StrDec : DecidableType
-    with Definition t := string
-    with Definition eq := fun (x y : string) => x = y.
-  Definition t := string.
-  Definition eq_dec := string_dec.
-  Definition eq (x y : string) := x = y.
-
-  Theorem eq_refl : forall x : t, eq x x.
-  Proof.
-    unfold eq.
-    intros.
-    reflexivity.
-  Qed.
-
-  Theorem eq_sym : forall x y : t, eq x y -> eq y x.
-  Proof.
-    unfold eq.
-    apply sym_eq.
-  Qed.
-
-  Theorem eq_trans : forall x y z : t, eq x y -> eq y z -> eq x z.
-  Proof.
-    unfold eq.
-    apply trans_eq.
-  Qed.
-End StrDec.
-
-Module TEnv := FMapWeakList.Make StrDec.
-Module TEnvWF := FMapFacts.WFacts_fun StrDec TEnv.
-Module TEnvProp := WProperties_fun StrDec TEnv.
-Definition tenv := TEnv.t type.
-Definition empty_env : tenv := TEnv.empty type.
+Definition tenv := table type.
+Definition empty := Table.empty type.
 
 Inductive Typed : term -> tenv -> type -> Prop :=
   | TVar    : forall (tenv : tenv) (s : string) (ty : type),
-                TEnv.MapsTo s ty tenv -> Typed (Var s) tenv ty
+                Table.MapsTo s ty tenv -> Typed (Var s) tenv ty
   | TBool   : forall (tenv : tenv) (b : bool) ,
                 Typed (Bool b) tenv BoolT
   | TLambda : forall (tenv : tenv) (x : string) (a b : type) (body : term),
-                Typed body (TEnv.add x a tenv) b -> Typed (Lambda x a body) tenv (FunT a b)
+                Typed body (Table.add x a tenv) b -> Typed (Lambda x a body) tenv (FunT a b)
   | TApply  : forall (tenv : tenv) (t1 t2 : term) (a b : type),
                 Typed t1 tenv (FunT a b) -> Typed t2 tenv a -> Typed (Apply t1 t2) tenv b
   | TIf     : forall (tenv : tenv) (t1 t2 t3 : term) (ty : type),
                 Typed t1 tenv BoolT -> Typed t2 tenv ty -> Typed t3 tenv ty ->
                    Typed (If t1 t2 t3) tenv ty.
+
+Lemma add_elim: forall t S T tenv s,
+    ~ FV s t -> Typed t (Table.add s S tenv) T -> Typed t tenv T.
+Proof.
+intro.
+induction t.
+ intros.
+ inversion H0.
+ apply TVar.
+ apply TableWF.add_mapsto_iff in H2.
+ inversion H2; inversion H5.
+  assert (FV s0 (Var s)).
+   rewrite H6 in |- *.
+   apply FVVar.
+
+   contradiction.
+
+  inversion H5.
+  exact H7.
+
+ intros.
+ inversion H0.
+ apply TBool.
+
+ intros.
+ inversion H0.
+ apply TLambda.
+ destruct (string_dec s s0).
+  rewrite <- (add_1 _ tenv0 s t S) in |- *.
+  rewrite <- e in H6.
+  trivial.
+
+  apply IHt with (S := S) (s := s0).
+   apply FV_Lambda_inv with (y := s) (T := t).
+    apply sym_not_eq.
+    trivial.
+
+    trivial.
+
+   apply (add_2 _ tenv0 s s0 t S) in n.
+   rewrite <- n in |- *.
+   trivial.
+
+ intros.
+ inversion H0.
+ apply TApply with (a := a).
+  apply IHt1 with (S := S) (s := s).
+   apply FV_Apply_inv_1 with (t2 := t2).
+   trivial.
+
+   trivial.
+
+  apply IHt2 with (S := S) (s := s).
+   apply FV_Apply_inv_2 with (t1 := t1).
+    trivial.
+
+    trivial.
+
+ intros.
+ inversion H0.
+ apply TIf.
+  apply IHt1 with (S := S) (s := s).
+   apply FV_If_inv_1 with (t2 := t2) (t3 := t3).
+   trivial.
+
+   trivial.
+
+  apply IHt2 with (S := S) (s := s).
+   apply FV_If_inv_2 with (t1 := t1) (t3 := t3).
+   trivial.
+
+   trivial.
+
+
+  apply IHt3 with (S := S) (s := s).
+   apply FV_If_inv_3 with (t1 := t1) (t2 := t2).
+   trivial.
+
+   trivial.
+
+Qed.
+
+Lemma add_intro: forall t S T tenv s,
+    ~ FV s t -> ~ BV s t -> Typed t tenv T -> Typed t (Table.add s S tenv) T.
+Proof.
+induction t.
+ intros.
+ apply TVar.
+ apply Table.add_2.
+  intro; apply H.
+  rewrite H2 in |- *.
+  apply FVVar.
+
+  inversion H1.
+  trivial.
+
+ intros.
+ inversion H1.
+ apply TBool.
+
+ intros.
+ inversion H1.
+ apply TLambda.
+ assert (s <> s0).
+  intro.
+  apply H0.
+  rewrite H8 in |- *.
+  apply BVLambda1.
+
+  generalize H8.
+  intro.
+  apply (add_2 _ tenv0 s s0 t S) in H8.
+  rewrite H8 in |- *.
+  apply IHt.
+   intro.
+   apply H.
+   apply FVLambda.
+    apply sym_not_eq.
+    trivial.
+
+    trivial.
+
+   intro.
+   apply H0.
+   apply BVLambda2.
+   trivial.
+
+   trivial.
+
+ intros.
+ inversion H1.
+ apply TApply with (a := a).
+  apply IHt1.
+   intro; apply H.
+   apply FVApply.
+   left; trivial.
+
+   intro; apply H0.
+   apply BVApply.
+   left; trivial.
+
+   exact H4.
+
+  apply IHt2.
+   intro; apply H.
+   apply FVApply.
+   right; trivial.
+
+   intro; apply H0.
+   apply BVApply.
+   right; trivial.
+
+   exact H7.
+
+ intros.
+ inversion H1.
+ apply TIf.
+  apply IHt1.
+   intro; apply H.
+   apply FVIf.
+   left; trivial.
+
+   intro; apply H0.
+   apply BVIf.
+   left; trivial.
+
+   exact H5.
+
+  apply IHt2.
+   intro; apply H.
+   apply FVIf.
+   right; left; trivial.
+
+   intro; apply H0.
+   apply BVIf.
+   right; left; trivial.
+
+   trivial.
+
+  apply IHt3.
+   intro; apply H.
+   apply FVIf.
+   right; right; trivial.
+
+   intro; apply H0.
+   apply BVIf.
+   right; right; trivial.
+
+   trivial.
+Qed.
