CannonicalForm.v
@@ -2,12 +2,13 @@ Require Import List.
 Require Import String.
 
 Require Import Term.
+Require Import Tables.
 Require Import Eval.
 Require Import Typing.
 
 Lemma bool_can :
   forall (v : term),
-    Value v -> Typed v empty_env BoolT ->
+    Value v -> Typed v empty BoolT ->
       v = Bool true \/ v = Bool false.
 Proof.
 intros.
@@ -23,12 +24,12 @@ Qed.
 
 Lemma lambda_can :
   forall (v : term) (ty1 ty2 : type),
-    Value v -> Typed v empty_env (FunT ty1 ty2) ->
+    Value v -> Typed v empty (FunT ty1 ty2) ->
       exists x : string, exists body : term, v = Lambda x ty1 body.
 Proof.
 intros.
 inversion H0.
- apply TEnv.empty_1 in H1.
+ apply Table.empty_1 in H1.
  contradiction .
 
  exists x.
