Subst.v
@@ -6,30 +6,28 @@ Require Import Eval.
 Require Import Alpha.
 Require Import AlphaFact.
 Require Import Typing.
-Require Import TypingFact.
+Require Import Tables.
 
 Lemma subst_preserve : forall t s x T S tenv,
-    Typed t (TEnv.add x S tenv) T -> Typed s tenv S -> Typed (subst t x s) tenv T.
+    Typed t (Table.add x S tenv) T -> Typed s tenv S -> Typed (subst t x s) tenv T.
 Proof.
 intros x0 s x.
 functional induction (subst x0 x s) .
- (* Var-1 *)
  intros.
  rewrite _x in H.
  inversion H.
- apply TEnvWF.add_mapsto_iff in H2.
+ apply TableWF.add_mapsto_iff in H2.
  inversion H2.
   inversion H5.
   rewrite <- H7 in |- *.
-  exact H0.
+  trivial.
 
   inversion H5.
   tauto.
 
- (* Var-2 *)
  intros.
  inversion H.
- apply TEnvWF.add_mapsto_iff in H2.
+ apply TableWF.add_mapsto_iff in H2.
  inversion H2.
   inversion H5.
   apply sym_eq in H6.
@@ -37,26 +35,20 @@ functional induction (subst x0 x s) .
 
   apply TVar.
   inversion H5.
-  exact H7.
+  trivial.
 
- (* Bool *)
  intros.
  inversion H.
  apply TBool.
 
- (* Lambda-1 *)
  intros.
  inversion H.
  apply TLambda.
  rewrite _x in H6.
- apply permutation with (tenv2 := TEnv.add x T tenv) in H6.
-  exact H6.
+ rewrite (add_1 _ tenv old T S) in H6.
+ rewrite _x in |- *.
+ trivial.
 
-  rewrite _x in |- *.
-  apply Equal_add_1.
-  reflexivity.
-
- (* Lambda-2 *)
  intros.
  inversion H.
  apply TLambda.
@@ -64,79 +56,45 @@ functional induction (subst x0 x s) .
   destruct (string_dec x (Flesh old new body)).
    rewrite <- e in |- *.
    rewrite alpha_id in |- *.
-   apply permutation with (tenv1 := TEnv.add x T (TEnv.add old S tenv)).
-    apply Equal_add_2.
-    exact _x.
+   generalize _x.
+   intro.
+   apply (add_2 _ tenv x old T S) in _x0.
+   rewrite <- _x0 in |- *.
+   trivial.
 
-    exact H6.
-
-   apply
-    permutation
-     with (tenv1 := TEnv.add (Flesh old new body) T (TEnv.add old S tenv)).
-    apply Equal_add_2.
-    apply sym_not_eq.
+   assert (old <> Flesh old new body).
     apply Flesh_x.
 
-    apply Typed_add_elim with (s := x) (S := T).
+    apply (add_2 _ tenv old (Flesh old new body) S T) in H7.
+    rewrite H7 in |- *.
+    apply add_elim with (s := x) (S := T).
      apply alpha_fv.
-     exact n.
+     trivial.
 
-     apply
-      permutation
-       with
-         (tenv1 := TEnv.add (Flesh old new body) T
-                     (TEnv.add x T (TEnv.add old S tenv))).
-      apply Equal_add_2.
-      apply sym_not_eq.
-      exact n.
+     apply (add_2 _ (Table.add old S tenv) x (Flesh old new body) T T) in n.
+     rewrite n in |- *.
+     apply alpha_preserve.
+      trivial.
 
-      apply alpha_preserve.
-       exact H6.
+      apply Flesh_fv2.
 
-       apply Flesh_fv2.
+      apply Flesh_bv2.
 
-       apply Flesh_bv2.
+      apply Table.add_1.
+      reflexivity.
 
-       apply TEnv.add_1.
-       reflexivity.
+  apply add_intro; [apply Flesh_fv1 | apply Flesh_bv1 | trivial].
 
-  apply Typed_add_intro.
-   apply Flesh_fv1.
-
-   apply Flesh_bv1.
-
-   exact H0.
-
- (* Apply *)
  intros.
  inversion H.
  apply TApply with (a := a).
-  apply IHt with (S := S).
-   exact H3.
+  apply IHt with (S := S); trivial.
+  apply IHt0 with (S := S); trivial.
 
-   exact H0.
-
-  apply IHt0 with (S := S).
-   exact H6.
-
-   exact H0.
-
- (* If *)
  intros.
  inversion H.
  apply TIf.
-  apply IHt with (S := S).
-   exact H4.
-
-   exact H0.
-
-  apply IHt0 with (S := S).
-   exact H7.
-
-   exact H0.
-
-  apply IHt1 with (S := S).
-   exact H8.
-
-   exact H0.
+  apply IHt with (S := S); trivial.
+  apply IHt0 with (S := S); trivial.
+  apply IHt1 with (S := S); trivial.
 Qed.
